replaced TM/Univ by top-level UTM construction (Universal, binary Turing machine with 1 tape)

theories/TM/Reductions/mTM_to_TM.v
@@ -1,6 +1,8 @@
 From Undecidability.TM Require Import Single.StepTM Code.CodeTM TM.
 Require Import Undecidability.Synthetic.Definitions.
 
+Set Default Goal Selector "!".
+
 Lemma nTM_to_MTM n :
   HaltTM n ⪯ HaltMTM.
 Proof.
@@ -13,20 +15,39 @@ Qed.
 
 Lemma mk_pTM n (sig : finType) (m : TM sig n) : pTM sig unit n.
 Proof.
-  unshelve econstructor. exact m. exact (fun _ => tt).
+  unshelve econstructor.
+  - exact m.
+  - exact (fun _ => tt).
 Defined. (* because definition *)
-
-Local Notation "[ s | p ∈ A ]" := (map (fun p => s) A) (p pattern).
 
 Definition enc_tape n Σ ls (t : Vector.t (tape Σ) n) :=
   [| midtape ls (inl START) (map inr (EncodeTapes.encode_tapes t) ++ [inl STOP]) |].
- 
-Lemma TM_sTM_simulation n Σ (M : TM Σ n) :
-  {M' : TM ((sigList (EncodeTapes.sigTape Σ)) ^+) 1 |
-      (forall q t t', eval M (start M) t q t' -> exists q, eval M' (start M') (enc_tape [] t) q (enc_tape [] t')) /\
-      (forall t, (exists q t', eval M' (start M') (enc_tape [] t) q t') -> (exists q t', eval M (start M) t q t')) }.
+
+Local Notation "[ s | p ∈ A ]" := (map (fun p => s) A) (p pattern).
+
+Section MTM_to_stM.
+
+Variables (n : nat) (sig : finType) (M : TM sig n) (ts : Vector.t (tape sig) n).
+
+Definition sig' := (sigList (EncodeTapes.sigTape sig)) ^+.
+Definition M' : TM sig' 1.
+Proof using M.
+  eapply mk_pTM in M.
+  destruct (ToSingleTape M) as [M' HM'].
+  exact M'.
+Defined.
+
+Definition ts' : Vector.t (tape sig') 1.
+Proof using ts.
+  eapply EncodeTapes.encode_tapes in ts.
+  pose (midtape nil (inl START) (map inr ts ++ [inl STOP])) as t'.
+  exact (Vector.cons _ t' _ (Vector.nil _)).
+Defined.
+
+Lemma TM_sTM_simulation' :
+  (forall q t t', eval M (start M) t q t' -> exists q, eval M' (start M') (enc_tape [] t) q (enc_tape [] t')) /\
+  (forall t, (exists q t', eval M' (start M') (enc_tape [] t) q t') -> (exists q t', eval M (start M) t q t')).
 Proof.
-  exists (projT1 (ToSingleTape (mk_pTM M))).
   split.
   - intros q t t'. repeat setoid_rewrite TM_eval_iff.
     intros [k H].
@@ -41,9 +62,10 @@ Proof.
       edestruct H2 as (t''' & [[q''' t''''] (k' & HH & <-)] & H3).
       + intros ? ? ? ?. exists outc, k0. eauto.
       + eapply H1.
-      + firstorder.
+      + firstorder easy.
       + eexists q'', _. unfold initc in H1.
-        etransitivity. eapply H1. repeat f_equal. 
+        etransitivity. { eapply H1. }
+        repeat f_equal. 
         eapply loop_injective in HH. 2: exact H. inv HH.
         unfold contains_tapes in H3. cbn in H3.
         destruct_tapes. cbn in *.
@@ -54,47 +76,35 @@ Proof.
     edestruct H0.
     * intros ? ? ? ?. exists outc, k0. eauto.
     * eapply H.
-    * firstorder.
+    * firstorder easy.
     * intuition. destruct H2 as (? & ? & ? & ?). subst.
       destruct x0 as [q'' t''].
       exists q'', t''. eapply TM_eval_iff. now exists x1.
+Qed.
+
+Lemma MTM_to_stM_correct : HaltsTM M ts <-> HaltsTM M' ts'.
+Proof.
+  unfold HaltsTM. split.
+  - intros [? [? [? ?]%TM_sTM_simulation']]. do 2 eexists. eassumption.
+  - now intros ?%TM_sTM_simulation'.
+Qed.
+
+End MTM_to_stM.
+
+Lemma TM_sTM_simulation n Σ (M : TM Σ n) :
+  {M' : TM ((sigList (EncodeTapes.sigTape Σ)) ^+) 1 |
+      (forall q t t', eval M (start M) t q t' -> exists q, eval M' (start M') (enc_tape [] t) q (enc_tape [] t')) /\
+      (forall t, (exists q t', eval M' (start M') (enc_tape [] t) q t') -> (exists q t', eval M (start M) t q t')) }.
+Proof.
+  exists (M' M). now apply TM_sTM_simulation'.
 Qed.
 
 Lemma MTM_to_stM :
   HaltMTM ⪯ HaltTM 1.
 Proof.
   unshelve eexists.
-  - intros [ [n sig] M t].
-    eapply mk_pTM in M. 
-    pose (ToSingleTape M). cbn in *.
-    eexists. destruct p. exact x.
-    cbn.
-    eapply EncodeTapes.encode_tapes in t.
-    econstructor. 2:econstructor.
-    refine (midtape nil (inl START) (map inr t ++ [inl STOP])).
-  - intros [ [n sig] M t]. cbn.
-    unfold HaltsTM.
-    setoid_rewrite TM_eval_iff.
-    intuition.
-    + destruct H as (q' & t' & k & H).
-      assert (M ↓ (fun t' k' => t = t' /\ k' = k)).
-      { intros ? ? []. subst. eauto. }
-      eapply (ToSingleTape_Terminates' (pM := mk_pTM M)) in H0.
-      specialize (H0 [|midtape [] (inl START) ([inr p | p ∈ EncodeTapes.encode_tapes t] ++ [inl STOP])|]).
-      edestruct H0. 
-      * exists t, k. repeat split; eauto.
-      * destruct x as [q'' t'']. exists q'', t''. 
-        destruct ((ToSingleTape (mk_pTM M))).
-        eexists.
-        eapply H1.
-    + destruct H as (q' & t' & k & H). cbn in *.
-      pose proof (ToSingleTape_Realise' (pM := mk_pTM M)).
-      specialize (H0 (fun t '(f,t') => exists outc k, loopM (initc M t) k = Some outc /\ ctapes outc = t')).
-      edestruct H0.
-      * intros ? ? ? ?. exists outc, k0. eauto.
-      * eapply H.
-      * firstorder.
-      * intuition. destruct H2 as (? & ? & ? & ?). subst.
-        destruct x0 as [q'' t''].
-        now exists q'', t'', x1.
+  { intros [[n sig] M ts].
+    exact (existT2 _ _ (sig' sig) (M' M) (ts' ts)). }
+  intros [[n sig] M ts].
+  apply MTM_to_stM_correct.
 Qed.
