theories/TM/Reductions/HaltTM_1_to_HaltSBTM.v
@@ -132,7 +132,7 @@ Qed.
 Theorem reduction :
   TM.HaltTM 1 ⪯ SBTM.HaltSBTM.
 Proof.
-  eapply reduces_transitive. eapply Arbitrary_to_Binary.reduction_tobin.
+  eapply reduces_transitive. eapply Arbitrary_to_Binary.reduction.
   unshelve eexists. { intros [M t]. refine (_, conv_tape t). refine (SBTM.Build_SBTM (num_states M) (@trans M)). }
   intros [M t]. split.
   - intros [q' [t' H]]. eapply red_correct1 in H.
