theories/TM/UTM.v
@@ -1,0 +1,29 @@
+(** * Halting problem for a fixed, universal, single-tape, binary Turing machine (HaltUTM) *)
+
+From Coq Require Import Vector.
+Import VectorNotations.
+
+From Undecidability Require Import TM Shared.Libs.PSL.FiniteTypes.FinTypesDef.
+
+From Undecidability Require
+  MinskyMachines.Reductions.KrivineMclosed_HALT_to_MMA_HALTING
+  TM.Reductions.MMA_HALTING_n_to_HaltTM_n
+  TM.Reductions.mTM_to_TM
+  TM.Reductions.Arbitrary_to_Binary.
+
+(* Universal, binary Turing machine with 1 tape *)
+Definition UTM : TM (finType_CS bool) 1.
+Proof.
+  (* universal Minsky machine with 5 registers *)
+  assert (MM5 := KrivineMclosed_HALT_to_MMA_HALTING.Argument.PROG 1).
+  (* universal Turing machine with 5 tapes *)
+  assert (TM5 := MMA_HALTING_n_to_HaltTM_n.Argument.P MM5).
+  (* universal Turing machine with 1 tape *)
+  assert (TM1 := mTM_to_TM.M' TM5).
+  (* universal, binary Turing machine with 1 tape *)
+  exact (Arbitrary_to_Binary.M' TM1).
+Defined.
+
+(* Given a binary tape t, does the machine UTM halt starting with t? *)
+Definition HaltUTM : tape (finType_CS bool) -> Prop :=
+  fun t => HaltsTM UTM [t].
